src/SMT_terms.v
@@ -641,9 +641,7 @@ Module Typ.
       apply cast_diff in H0.
       rewrite H in H0. inversion H0.
     Qed.
-        
-    
-    
+
     Lemma neq_cast : forall A B,
       cast A B = (if eqb A B then cast A B else NoCast).
     Proof.
@@ -1042,7 +1040,7 @@ Qed.
   
   Lemma eqb_spec : forall t1 t2, eqb t1 t2 <-> t1 = t2.
   Proof.
-    intros;symmetry;apply reflect_iff;apply reflect_eqb.
+    intros;symmetry; apply reflect_iff; apply reflect_eqb.
   Qed.
   
   (** Typing and interpretation *)
@@ -2645,6 +2643,55 @@ Qed.
 End Atom.
 
 Arguments Atom.Val {_} {_} _ _.
+
+Section ReflectFacts.
+
+Infix "-->" := implb (at level 60, right associativity) : bool_scope.
+
+Lemma reflect_iff : forall P b, reflect P b -> (P<->b=true).
+Proof.
+ intros; destruct H; easy.
+Qed.
+
+Lemma iff_reflect : forall P b, (P<->b=true) -> reflect P b.
+Proof.
+ intros.
+ destr_bool; constructor; try now apply H.
+ unfold not. intros. apply H in H0. destruct H. easy.
+Qed.
+
+Lemma reflect_dec : forall P b, reflect P b -> {P} + {~P}.
+Proof. intros; destruct H; [now left | now right]. Qed.
+
+ Lemma implyP : forall (b1 b2: bool), reflect (b1 -> b2) (b1 --> b2).
+ Proof. intros; apply iff_reflect; split;
+        case_eq b1; case_eq b2; intros; try easy; try compute in *; now apply H1.
+ Qed.
+
+ Lemma andP : forall (b1 b2: bool), reflect (b1 /\ b2) (b1 && b2).
+ Proof. intros; apply iff_reflect; split;
+        case_eq b1; case_eq b2; intros; try easy; try compute in *; now apply H1.
+ Qed.
+
+ Lemma orP : forall (b1 b2: bool), reflect (b1 \/ b2) (b1 || b2).
+ Proof. intros; apply iff_reflect; split;
+        case_eq b1; case_eq b2; intros; try easy; try compute in *.
+        destruct H1 as [H1a | H1b ]; easy. left. easy. left. easy.
+        right. easy.
+ Qed.
+
+ Lemma negP : forall (b: bool), reflect (~ b) (negb b).
+ Proof. intros; apply iff_reflect; split;
+        case_eq b; intros; try easy; try compute in *.
+        contradict H0. easy.
+ Qed.
+
+ Lemma eqP : forall (b1 b2: bool), reflect (b1 = b2) (Bool.eqb b1 b2).
+ Proof. intros; apply iff_reflect; split;
+        case_eq b1; case_eq b2; intros; try easy; try compute in *; now apply H1.
+ Qed.
+
+End ReflectFacts.
 
 (* These definitions are not used. This is just a hack, Coq refuses to
    construct PArrays from OCaml if these are not here for some silly reason *)
